src/polyfix.lean
@@ -1,10 +1,11 @@
 import polycodable
 import npolynomial
 import promise
+import polysize
 
 variables {α β : Type*}
 
-open polycodable (encode decode)
+open ptree.pencodable (encode decode)
 
 theorem fix_time_le {c : code} {x₀ : ptree} {N : ℕ} (b₁ b₂ : ℕ → ℕ) (mb : monotone b₁) 
   (h₁ : time_bound c b₁) (h₂ : ∀ {x : ptree}, x ∈ (c.fix_iterator x₀).states → x.sizeof ≤ b₂ x₀.sizeof) 
@@ -30,76 +31,187 @@ begin
   refine ⟨t, ht, t_le.trans _⟩, mono*; exact zero_le',
 end
 
--- theorem polytime_fix {c init : code} (pc : polytime c) (pinit : polytime init)
---   (hs : ∃ p : polynomial ℕ, ∀ {x : ptree}, )
-
--- safe: flip f : ((s, hd) : σ × α) → (acc : β) → β
--- safe (λ s ⟨acc, l⟩, (flip f) (s, l.head) acc)
-
-#exit
-
-theorem polytime_fix {c : code} (pc : polytime c) (p q : polynomial ℕ) (he : ∀ x : ptree, ∃ t ≤ p.eval x.sizeof, t ∈ time_iter ((c.eval.map ptree.to_option).res_inter {s | s.sizeof ≤ q.eval x.sizeof}) (pfun.pure 1) x) :
-  polytime c.fix :=
+theorem polytime_fix {c init : code} (pc : polytime c) (pinit : polytime init)
+  (hs : ∃ p : polynomial ℕ, ∀ {x₀ x : ptree}, x ∈ (c.fix_iterator (pinit.to_fun x₀)).states → x.sizeof ≤ p.eval (pinit.to_fun x₀).sizeof)
+  (hn : ∃ q : polynomial ℕ, ∀ (x₀ : ptree), ∃ N ∈ (c.fix_iterator (pinit.to_fun x₀)).time (pfun.pure 1), N ≤ q.eval (pinit.to_fun x₀).sizeof) :
+  polytime (c.fix.comp init) :=
 begin
-  rcases pc with ⟨f, f_le⟩, use p * (f.comp q) + polynomial.monomial 1 1, simp,
-  exact time_bound_fix (λ n, f.eval n) (λ n, q.eval n) (λ n, p.eval n) (monotone_polynomial_nat _) f_le he,
+  have ran_eq : init.eval.ran = set.range pinit.to_fun,
+  { ext, simp [pfun.mem_ran_iff, part.get_eq_iff_mem], },
+  simpa [← ran_eq, pinit.dom_univ] using polytime_promise_comp (polytime_fix_on_pred pc (set.range pinit.to_fun) _ _) (polytime_promise.univ.mpr pinit),
+  { cases hs with p hs, use p, rintros x₀ x' ⟨x, rfl⟩ hx', exact hs hx', },
+  { cases hn with q hn, use q, rintros x₀ ⟨x, rfl⟩, apply hn, },
 end
 
-theorem code.fix_respects [polycodable α] (c : code) (f : α →. option α) (sc : ∀ x, c.eval x = (f (decode x)).map encode) :
-  part_eval.fcommutes f (c.eval.map ptree.to_option) encode :=
-{ dom_of_dom := λ x, by { specialize sc (encode x), apply_fun part.dom at sc, simp at sc, simp [sc, pfun.map], },
-  some_of_some := λ a b h, by { specialize sc (encode a), simp [pfun.map, sc, part.eq_some_iff.mpr h, encode], },
-  none_of_none := λ a h, by { specialize sc (encode a), simp [pfun.map, sc, part.eq_some_iff.mpr h, encode], } }
+-- @[simps]
+def mk_iterator {α} (f : α →. bool × α) (x₀ : bool × α) : execution (bool × α) :=
+{ next := λ x, if x.1 = tt then (part.some none) else ((f x.2).map some),
+  start := x₀ }
 
-theorem code.fix_respects' [polycodable α] (c : code) (f : α →. option α) (sc : ∀ x, c.eval x = (f (decode x)).map encode) :
-  part_eval.fcommutes (c.eval.map ptree.to_option) f decode :=
-{ dom_of_dom := λ x, by { specialize sc x, apply_fun part.dom at sc, simp at sc, simp [sc, pfun.map], },
-  some_of_some := λ a b h, by { specialize sc a, simp [pfun.map, sc] at h, rcases h with ⟨a', h₁, h₂, rfl⟩, cases a', { contradiction, }, simpa [encode, ptree.of_option], },
-  none_of_none := λ a h, by { specialize sc a, simp [pfun.map, sc] at h, rcases h with ⟨a', h₁, h₂⟩, cases a', assumption, { contradiction, },  } }
+@[simp] lemma mk_iterator_some {f : α →. bool × α} {x₀ x x' : bool × α} :
+  some x' ∈ (mk_iterator f x₀).next x ↔ x.1 = ff ∧ x' ∈ f x.2 :=
+by { simp only [mk_iterator], split_ifs with h, { simp [h], }, rw bool_iff_false at h, simp [-prod.exists, h, and_comm], }
 
-lemma polytime.bdd_size_decode_encode (α : Type*) [polycodable α] :
-  ∃ (p : polynomial ℕ), ∀ x, (encode (decode x : α)).sizeof ≤ p.eval x.sizeof :=
+@[simp] lemma mk_iterator_none {f : α →. bool × α} {x₀ x : bool × α} :
+  none ∈ (mk_iterator f x₀).next x ↔ x.1 = tt :=
+by { simp only [mk_iterator], split_ifs with h; simp [h], }
+
+@[simp] lemma mk_iterator_dom {f : α →. bool × α} {x₀ x : bool × α} :
+  ((mk_iterator f x₀).next x).dom ↔ x.1 = tt ∨ (f x.2).dom :=
+by simp [mk_iterator, apply_ite part.dom]
+
+@[simp] lemma mk_iterator_start {f : α →. bool × α} {x₀ : bool × α} : (mk_iterator f x₀).start = x₀ := rfl
+
+@[simp] lemma mk_iterator_change_start {f : α →. bool × α} {x₀ x₀' : bool × α} :
+  (execution.mk (mk_iterator f x₀).next x₀') = (mk_iterator f x₀') :=
+by { ext : 1; simp, refl, } 
+
+@[simp] lemma some_eq_ite_none_some {α} (P : Prop) [decidable P] (a b : α) :
+  (some a = if P then none else some b) ↔ ¬P ∧ a = b :=
+by { split_ifs; simp; tauto, }
+
+@[simp] lemma none_eq_ite_none_some {α} (P : Prop) [decidable P] (b : α) :
+  (none = if P then none else some b) ↔ P := by { split_ifs; simpa, }
+
+@[simps]
+def code.fix_respects [ptree.pencodable α] (c : code) (f : α → bool × α) (sc : ∀ x : bool × α, c.eval (encode x) = part.some (encode (f x.2))) (x₀ : bool × α) :
+  (mk_iterator ↑f x₀) ∼ₛ (c.fix_iterator (encode x₀)) :=
+{ rel := λ x ex, ex = encode x,
+  dom_iff := λ _ _ _ _, by { rintro rfl, conv_lhs { simp, }, conv_rhs { simp [code.fix_iterator, sc, apply_ite part.dom], }, },
+  some_iff := λ x ex x' ex' _ _, by { rintro rfl, cases x, simp [sc], rintros rfl rfl _, exact id, },
+  none_iff := λ x ex hx hex, by { rintro rfl, cases x with x₁ x₂, simp [encode], cases x₁; simp, },
+  start := rfl }
+
+theorem polytime_fun.eval' {α β} [polycodable α] [polycodable β] (f : α → bool × α) (init : β → bool × α)
+  (hf : polytime_fun f) (hinit : polytime_fun init)
+  (hs : ∃ p : polynomial ℕ, ∀ {x₀ x}, x ∈ (mk_iterator ↑f (init x₀)).states → (encode x).sizeof ≤ p.eval (encode $ init x₀).sizeof)
+  (hn : ∃ q : polynomial ℕ, ∀ x₀, ∃ N ∈ (mk_iterator ↑f (init x₀)).time (pfun.pure 1), N ≤ q.eval (encode $ init x₀).sizeof)
+  (g : β → α) (hg : ∀ x, (tt, g x) ∈ (mk_iterator ↑f (init x)).eval) : polytime_fun g :=
 begin
-  obtain ⟨c, ⟨p, hp⟩, sc⟩ := polycodable.polytime_decode α, use p,
-  intro x, specialize sc x, specialize hp x, rcases hp with ⟨t, H, t_le⟩,
-  have := eval_sizeof_le_time (part.eq_some_iff.mp sc) H, exact this.trans t_le,
+  suffices : polytime_fun (λ x, (tt, g x)), { exact polytime_fun.snd.comp this, },
+  obtain ⟨c, pc, sc⟩ : polytime_fun (λ x : bool × α, f x.2) := by polyfun,
+  let R := code.fix_respects c f sc,
+  rw polytime_fun_iff at hinit, rcases hinit with ⟨ci, pci, sci⟩,
+  use c.fix.comp ci, split,
+  { apply polytime_fix pc pci,
+    { cases hs with p hs, simp [sci],
+      use p, intros x₀ x hx, 
+      obtain ⟨x, hy, hrel⟩ := (R (init (decode x₀))).symm.exists_state_of hx,
+      simp at hrel, subst hrel, exact hs hy, },
+    { cases hn with q hn, simp [sci], 
+      use q, intros x₀, specialize R (init (decode x₀)), specialize hn (decode x₀),
+      simpa [R.time_pure_eq] using hn, } },
+  intro x, simp [sci], rw ← code.fix_iterator,
+  simpa [part.eq_some_iff] using (R (init x)).mem_eval_of (hg x),
 end
 
-theorem polytime_fun.eval' [polycodable α] (f : α → option α) (g : α → α) (hf : polytime_fun f) (p q : polynomial ℕ)
-  (hg : ∀ x, g x ∈ eval (f : α →. option α) x) (H : ∀ x : α, ∃ t ≤ p.eval (encode x).sizeof, t ∈ time_iter (pfun.res f {s : α | (encode s).sizeof ≤ q.eval (encode x).sizeof}) (pfun.pure 1) x) :
-  polytime_fun g :=
+@[simps]
+def curry_state {α β} (f : β → α → bool × α) (x : β) (y : bool × α) :
+  (mk_iterator ↑(f x) y) ∼ₛ (mk_iterator ↑(λ x' : β × α, ((f x'.1 x'.2).1, x'.1, (f x'.1 x'.2).2)) (y.1, x, y.2)) :=
+{ rel := λ a b, b = (a.1, x, a.2),
+  dom_iff := by { intros, simp, },
+  some_iff := λ a b a' b' _ _, by { rintro rfl, simp, rintros _ rfl _ rfl, refl, },
+  none_iff := λ a a' _ _, by { rintro rfl, simp, },
+  start := rfl }
+
+theorem polytime_fun.eval {α β} [polycodable α] [polycodable β] {f : β → α → bool × α} {init : β → bool × α}
+  (hf : polytime_fun₂ f) (hinit : polytime_fun init)
+  (hs : ∃ p : polynomial ℕ, ∀ {x₀ x}, x ∈ (mk_iterator ↑(f x₀) (init x₀)).states → (encode x).sizeof ≤ p.eval (encode x₀).sizeof)
+  (hn : ∃ q : polynomial ℕ, ∀ x₀, ∃ N ∈ (mk_iterator ↑(f x₀) (init x₀)).time (pfun.pure 1), N ≤ q.eval (encode x₀).sizeof)
+  (g : β → α) (hg : ∀ x, (tt, g x) ∈ (mk_iterator ↑(f x) (init x)).eval) : polytime_fun g :=
 begin
-  rw polytime_fun_iff at hf, rcases hf with ⟨c, pc, sc⟩,
-  use c.fix, split, swap,
-  { intro x, simp, have := part_eval.frespects.eval_eq (c.fix_respects (f : α →. option α) _).to_frespects,
-    simp [this, part.eq_some_iff.mpr (hg x)], simp [sc], },
-  obtain ⟨P, hP⟩ := polytime.bdd_size_decode_encode α,
-  apply polytime_fix pc (p.comp P) ((q.comp P) + polynomial.monomial 1 1),
-  intro x, rcases H (decode x) with ⟨t, ht, t_mem⟩, refine ⟨t, ht.trans _, _⟩,
-  { simp, apply monotone_polynomial_nat, apply hP, },
-  have := code.fix_respects' c (f : α →. option α) _, swap, { simp [sc], }, 
-  have T := λ S : set α, part_eval.eq_time_of_fcommutes (this.restrict S), simp at T, rw ← T at t_mem,
-  rw part_eval.time_iter_invariant ({x} ∪ set.range (@encode α _)) at t_mem, simp at t_mem,
-  apply part_eval.time_iter_mono _ t_mem,
-  { intros x' y', simp, refine λ h₁ h₂ h₃, ⟨_, h₃⟩, rcases h₂ with rfl|⟨y, rfl⟩, { simp, },
-    simp at h₁, apply le_add_right, refine h₁.trans _, apply monotone_polynomial_nat, apply hP, },
-  { intros x' y' _, simp [sc, pfun.map], intros _ H₃, right, simp [encode] at H₃, rcases H₃ with ⟨y₂, _, rfl⟩, use y₂, },
+  suffices : polytime_fun (λ x : β, (x, g x)), { apply polytime_fun.snd.comp this, },
+  let R := curry_state f,
+  apply polytime_fun.eval' (λ x : β × α, ((f x.1 x.2).1, x.1, (f x.1 x.2).2)) (λ x : β, ((init x).1, x, (init x).2)),
+  { polyfun, }, { polyfun, },
+  { cases hs with p hs, use p + polynomial.monomial 1 1, 
+    rintros x₀ ⟨b, x₀', s⟩ H,
+    obtain ⟨⟨b', s'⟩, h₁, h₂⟩ := (R x₀ (init x₀)).symm.exists_state_of H,
+    simp at h₂, rcases h₂ with ⟨rfl, rfl, rfl⟩,
+    specialize hs h₁, simp at hs ⊢, 
+    ac_change ((encode b).sizeof + (encode s).sizeof + 1) + ((encode x₀').sizeof + 1) ≤ _,
+    mono, { refine hs.trans _, apply monotone_polynomial_nat, linarith only, }, { linarith only, }, },
+  { cases hn with q hn, use q, intros x₀,
+    simp_rw (R x₀ (init x₀)).symm.time_pure_eq,
+    rcases hn x₀ with ⟨N, h, N_le⟩, refine ⟨N, h, N_le.trans _⟩,
+    simp, apply monotone_polynomial_nat, linarith only, },
+  intro x,
+  obtain ⟨⟨r₁, r₂, r₃⟩, hr₁, hr₂⟩ := (R x (init x)).mem_eval_of (hg x),
+  simp at hr₂, rcases hr₂ with ⟨rfl, rfl, rfl⟩, exact hr₁,
+end
+
+noncomputable theory
+open_locale classical
+
+noncomputable instance {σ : Type*} [polycodable σ] (f : execution σ) : ptree.pencodable f.states :=
+set_encodable _ f.start_mem_states
+
+theorem polytime_fun.eval_of_polysize {α β} [polycodable α] [polycodable β] {f : β → α → bool × α} {init : β → bool × α}
+  (hf : polytime_fun₂ f) (hinit : polytime_fun init)
+  (hfs : polysize_fun_safe (λ (x₀ : β) (y : (mk_iterator ↑(f x₀) (init x₀)).states), f x₀ (y : bool × α).2))
+  (hn : ∃ q : polynomial ℕ, ∀ x₀, ∃ N ∈ (mk_iterator ↑(f x₀) (init x₀)).time (pfun.pure 1), N ≤ q.eval (encode x₀).sizeof) 
+  (g : β → α) (hg : ∀ x, (tt, g x) ∈ (mk_iterator ↑(f x) (init x)).eval) : polytime_fun g :=
+begin
+  refine polytime_fun.eval hf hinit _ hn g hg,
+  rcases hfs with ⟨p, hp⟩, rcases hn with ⟨q, hn⟩, dsimp only at hp,
+  obtain ⟨p₂, hp₂⟩ := polysize_of_polytime_fun hinit,
+  use p₂ + p * q, intros x₀,
+  suffices : ∀ (s : ℕ × bool × α), s ∈ ((mk_iterator ↑(f x₀) (init x₀)).time_with (pfun.pure 1)).states → (encode s.2).sizeof ≤ p₂.eval (encode x₀).sizeof + (p.eval (encode x₀).sizeof) * s.1,
+  { intros s hs, 
+    obtain ⟨⟨t, s'⟩, h₁, h₂⟩ := (execution.time_with_tr (mk_iterator ↑(f x₀) (init x₀)) (pfun.pure 1) (by simp)).exists_state_of hs,
+    simp at h₂, subst h₂,
+    specialize this _ h₁, specialize hn x₀, specialize hp x₀, simp at this ⊢,
+    refine this.trans _,
+    mono*, any_goals { exact zero_le' },
+    rcases hn with ⟨N, hN, N_le⟩,
+    exact (execution.state_time_le_time _ _ hN h₁).trans N_le, },
+  intros s hs, apply execution.step_induction hs,
+  { specialize hp₂ x₀, simpa [execution.time_with], },
+  rintros ⟨t, s⟩ ⟨t', s'⟩ hs ih,
+  simp [execution.time_with, ← apply_ite part.some],
+  rintros rfl _ rfl,
+  specialize hp x₀ ⟨s, _⟩,
+  { obtain ⟨⟨_, s'⟩, h₁, h₂⟩ := (execution.time_with_tr (mk_iterator ↑(f x₀) (init x₀)) (pfun.pure 1) (by simp)).symm.exists_state_of hs, simp at h₂, rwa ← h₂, },
+  refine hp.trans _, rw [add_comm 1 t, mul_add], simp [← add_assoc], 
+  exact ih.trans rfl.le,
+end
+
+@[simp]
+def iterator_evaln {α : Type*} (f : α → bool × α) : ℕ → bool × α → option α
+| 0 _ := none
+| (n+1) (b, x) := cond b (some x) (iterator_evaln n (f x))
+
+lemma eval_of_iterator_evaln {α} {f : α → bool × α} {N : ℕ} {x₀ : bool × α} {y : α}
+  (hy : y ∈ iterator_evaln f N x₀) : ∃ n ≤ N, (n, tt, y) ∈ ((mk_iterator ↑f x₀).time_with (pfun.pure 1)).eval :=
+begin
+  induction N with N ih generalizing x₀, { contradiction, },
+  cases x₀ with b₀ x₀,
+  cases b₀, swap,
+  { refine ⟨0, zero_le', _⟩, rw [execution.time_with, execution.mem_eval],
+    simp at hy, subst hy, split, { exact execution.start_mem_states _, }, simp, },
+  simp at hy, specialize ih hy, rcases ih with ⟨n, H, n_mem⟩,
+  refine ⟨n+1, _, _⟩, { simpa [nat.succ_eq_add_one], },
+  rw ← @execution.eval_from _ _ (1, f x₀), swap,
+  { apply execution.mem_states_of_fwd (execution.start_mem_states _), simp [execution.time_with], },
+  simp only [execution.time_with], rw track_with_change_start,
   simp,
+  have := (mk_iterator ↑f (f x₀)).time_fwd (pfun.pure 1) 1, simp at this, rw this,
+  rw ← part.eq_some_iff at n_mem, simp [n_mem],
 end
 
-theorem polytime_fun.eval [polycodable α] [polycodable β]
-  (f : β → α → option α) (g : β → α → α) (hf : polytime_fun₂ f) (p q : polynomial ℕ)
-  (hg : ∀ s x, g s x ∈ eval (f s : α →. option α) x)
-  (H : ∀ S x, ∃ t ≤ p.eval (encode (S, x)).sizeof, t ∈ time_iter (pfun.res (f S) {s : α | (encode (S, s)).sizeof ≤ q.eval (encode (S, x)).sizeof}) (pfun.pure 1) x) :
-  polytime_fun₂ g :=
+theorem polytime_fun.evaln_of_polysize {α β} [polycodable α] [polycodable β] {f : β → α → bool × α} {init : β → bool × α}
+  (hf : polytime_fun₂ f) (hinit : polytime_fun init) (N : β → ℕ)
+  (hfs : polysize_fun_safe (λ (x₀ : β) (y : (mk_iterator ↑(f x₀) (init x₀)).states), f x₀ (y : bool × α).2))
+  (hn : ∃ q : polynomial ℕ, ∀ x₀, N x₀ ≤ q.eval (encode x₀).sizeof) 
+  (g : β → α) (hg : ∀ x, g x ∈ iterator_evaln (f x) (N x) (init x)) : polytime_fun g :=
 begin
-  have HR : ∀ S : β, part_eval.fcommutes (f S : α →. option α) (λ s : β × α, (f s.1 s.2).map (prod.mk s.1)) (λ x, (S, x)),
-  { refine λ S, ⟨_, _, _⟩, { simp, }, { simp, exact λ _ _ h, h.symm, }, { simp, }, },
-  have := polytime_fun.eval' (λ s : β × α, (f s.1 s.2).map (λ r, (s.1, r))) (λ s, (s.1, g s.1 s.2)) _ p q _ _,
-  { apply polytime_fun.comp polytime_fun.snd this, },
-  { polyfun, },
-  { rintro ⟨x₀, x₁⟩, simp, rw (HR x₀).to_frespects.eval_eq x₁, simp, apply hg, },
-  rintro ⟨x₀, x₁⟩, rcases H x₀ x₁ with ⟨t, ht, t_mem⟩, use [t, ht],
-  have HR' := (HR x₀).restrict {s : β × α | (encode s).sizeof ≤ q.eval (encode (x₀, x₁)).sizeof}, simp at HR',
-  rw ← part_eval.eq_time_of_fcommutes HR', exact t_mem,
+  refine polytime_fun.eval_of_polysize hf hinit hfs _ g _,
+  { rcases hn with ⟨q, hn⟩, use q, intros x₀, 
+    obtain ⟨n, n_le, hn'⟩ := eval_of_iterator_evaln (hg x₀),
+    use n, refine ⟨_, n_le.trans (hn _)⟩,
+    simp only [execution.time], rw ← part.eq_some_iff at hn', simp [hn'], },
+  intros x₀,
+  obtain ⟨_, _, hn'⟩ := eval_of_iterator_evaln (hg x₀),
+  obtain ⟨y, hy, hrel⟩ := (execution.time_with_tr (mk_iterator ↑(f x₀) (init x₀)) (pfun.pure 1) (by simp)).symm.mem_eval_of hn',
+  simp at hrel, rwa ← hrel,
 end
