src/polysize.lean
@@ -1,9 +1,11 @@
 import polycodable
 
-variables {α β γ δ ε : Type*} [polycodable α] [polycodable β] [polycodable γ]
- [polycodable δ] [polycodable ε]
+open ptree (pencodable)
 
-open polycodable (encode)
+variables {α β γ δ ε : Type*} [pencodable α] [pencodable β] [pencodable γ]
+ [pencodable δ] [pencodable ε]
+
+open ptree.pencodable (encode decode)
 
 @[simp] lemma encode_sizeof_ptree (x : ptree) : (encode x).sizeof = x.sizeof := rfl
 lemma one_le_encode_sizeof (x : α) :
@@ -12,6 +14,51 @@ by { cases (encode x); simp, linarith only, }
 
 @[simp] lemma encode_sizeof_pair (a : α) (b : β) : (encode (a, b)).sizeof = (encode a).sizeof + (encode b).sizeof + 1 :=
 by { simp [encode], ac_refl, }
+
+
+@[simp] lemma encode_sizeof_nil : (encode ([] : list γ)).sizeof = 1 :=
+by simp [encode]
+@[simp] lemma encode_sizeof_cons (a : γ) (b : list γ) :
+  (encode (a :: b)).sizeof = 1 + (encode a).sizeof + (encode b).sizeof :=
+by simp [encode]
+
+lemma encode_sizeof_le_of_mem {l : list γ} {x : γ} (hx : x ∈ l) :
+  (encode x).sizeof ≤ (encode l).sizeof :=
+begin
+  induction l with hd tl ih, { simp at hx, contradiction, },
+  rcases ((list.mem_cons_iff _ _ _).mp hx) with rfl|h; simp,
+  { linarith only, },
+  linarith only [ih h],
+end
+
+@[simp] lemma encode_sizeof_append (a b : list γ) :
+  ((encode (a ++ b)).sizeof : ℤ) = ((encode a).sizeof : ℤ) + (encode b).sizeof - 1 :=
+by { induction a with hd tl ih, { simp, }, simp [ih], ring, }
+
+lemma encode_sizeof_le_of_sublist {a b : list γ} (h : a <+ b) :
+  (encode a).sizeof ≤ (encode b).sizeof :=
+begin
+  induction h, { simp, },
+  case list.sublist.cons : l₁ l₂ s₁ H ih { refine ih.trans _, simp, },
+  case list.sublist.cons2 : l₁ l₂ s₁ H ih { simpa, },
+end
+
+lemma encode_sizeof_le_of_infix {a b : list γ} (h : a <:+: b) :
+  (encode a).sizeof ≤ (encode b).sizeof :=
+encode_sizeof_le_of_sublist h.sublist
+
+lemma encode_list_sizeof (l : list γ) : 
+  (encode l).sizeof = (l.map (λ x, (encode x).sizeof)).sum + l.length + 1 :=
+by { induction l with hd tl ih, { simp, }, simp [ih], ac_refl, }
+
+@[simp] lemma encode_sizeof_reverse (l : list γ) :
+  (encode l.reverse).sizeof = (encode l).sizeof :=
+by { simp [encode_list_sizeof, list.sum_reverse], }
+
+lemma len_le_encode_sizeof (a : list γ) :
+  a.length + 1 ≤ (encode a).sizeof :=
+by { induction a with hd tl ih, { simp, }, simp, linarith, }
+
 
 def polysize_fun (f : α → β) : Prop :=
 ∃ p : polynomial ℕ, ∀ (x : α), (encode (f x)).sizeof ≤ p.eval (encode x).sizeof
@@ -58,32 +105,55 @@ polysize_fun.comp hf (polysize_fun.pair hg (polysize_fun.pair hh hi))
 
 lemma polysize_fun_of_fin_range [fintype β] (f : α → β) : polysize_fun f :=
 begin
-  haveI : nonempty β := ⟨polycodable.decode ptree.nil⟩,
+  haveI : nonempty β := ⟨decode ptree.nil⟩,
   let B := ((finset.image (λ x : β, (encode x).sizeof) finset.univ).max' _ : ℕ),
   { use B, intro x, simp, apply finset.le_max', simp, },
   simpa using finset.univ_nonempty,
 end
 
-def polysize_fun_safe (f : α → β → γ) : Prop :=
-∃ p : polynomial ℕ, ∀ (x : α) (y : β), (encode (f x y)).sizeof ≤ (encode y).sizeof + p.eval (encode x).sizeof
+variables {σ : α → Type*} [∀ x, pencodable (σ x)]
+def polysize_fun_safe (f : Π x, (σ x) → γ) : Prop :=
+∃ p : polynomial ℕ, ∀ (x : α) (y : σ x), (encode (f x y)).sizeof ≤ (encode y).sizeof + p.eval (encode x).sizeof
 
-lemma polysize_fun_safe_iff_polysize {f : α → γ} :
+lemma polysize_fun_safe_of_polysize {f : α → γ} :
+  polysize_fun f → polysize_fun_safe (λ x (_ : σ x), f x)
+| ⟨p, hp⟩ := by { refine ⟨p, λ _ _, (hp _).trans _⟩, simp, }
+
+@[simp] lemma polysize_fun_safe_iff_polysize {f : α → γ} :
   polysize_fun_safe (λ x (_ : β), f x) ↔ polysize_fun f :=
 begin
-  split,
-  { inhabit β, 
-    rintro ⟨p, hp⟩,
-    use p + (encode (default : β)).sizeof, intro x,
-    simpa [add_comm] using hp x default, },
-  { rintro ⟨p, hp⟩,
-    refine ⟨p, λ _ _, (hp _).trans _⟩,
-    simp, }
+  split, swap, { exact polysize_fun_safe_of_polysize, },
+  inhabit β, 
+  rintro ⟨p, hp⟩, dsimp only at hp,
+  use p + (encode (default : β)).sizeof, intro x,
+  simpa [add_comm] using hp x default,
 end
 
-lemma polysize_fun_safe.comp {δ ε : Type*} [polycodable δ] [polycodable ε]
-  {f : α → β → γ} {g : δ → α} {h : δ → ε → β} :
-  polysize_fun_safe f → polysize_fun g → polysize_fun_safe h →
-  polysize_fun_safe (λ x y, f (g x) (h x y))
+def polysize_fun_uniform (f : Π x, (σ x) → γ) : Prop :=
+∃ p : polynomial ℕ, ∀ (x : α) (y : σ x), (encode (f x y)).sizeof ≤ p.eval (encode x).sizeof
+
+@[simp] lemma polysize_fun_uniform_iff_polysize {f : α → γ} :
+  polysize_fun_uniform (λ x (_ : σ x), f x) ↔ polysize_fun f :=
+begin
+  split,
+  { rintro ⟨p, hp⟩, use p, intro x, inhabit (σ x),
+    simpa using hp x default, },
+  { rintro ⟨p, hp⟩, exact ⟨p, λ _ _, (hp _).trans rfl.le⟩ },
+end
+
+lemma polysize_fun_uniform.pair {f : Π x, (σ x) → β} {g : Π x, (σ x) → γ} :
+  polysize_fun_uniform f → polysize_fun_uniform g → polysize_fun_uniform (λ x y, (f x y, g x y))
+| ⟨pf, hpf⟩ ⟨pg, hpg⟩ :=
+begin
+  use pf + pg + 1,
+  intros x y,
+  simp, mono,
+end
+
+lemma polysize_fun_safe.comp {δ : Type*} {ε : δ → Type*} [pencodable δ] [∀ x, pencodable (ε x)]
+  {f : α → β → γ} {g : Π x, ε x → α} {h : Π x, ε x → β} :
+  polysize_fun_safe f → polysize_fun_uniform g → polysize_fun_safe h →
+  polysize_fun_safe (λ x y, f (g x y) (h x y))
 | ⟨pf, hf⟩ ⟨pg, hg⟩ ⟨ph, hh⟩ :=
 begin
   use ph + (pf.comp pg),
@@ -92,11 +162,8 @@ begin
   simp [← add_assoc], mono*,
 end
 
-instance : polycodable (list α) := sorry
-
-example {σ : Type*} [polycodable σ] [inhabited α] {f : σ × α → β → β} (hf : polysize_fun_safe f) :
-  polysize_fun_safe (λ (s : σ) (acc : β × list α), f (s, acc.2.head) acc.1) :=
-begin
-  
-end
-
+def set_encodable (S : set α) [decidable_pred (∈ S)] {d : α} (hd : d ∈ S) : ptree.pencodable S :=
+ptree.pencodable.mk'
+(coe : S → α)
+(λ x, if h : x ∈ S then ⟨x, h⟩ else ⟨d, hd⟩)
+(λ x, by simp) 
